src/HOL/SET-Protocol/MessageSET.thy
@@ -835,13 +835,8 @@ subsection{*Tactics useful for many protocol proofs*}
 (*<*)
 ML
 {*
-val analz_increasing = thm "analz_increasing";
-val analz_subset_parts = thm "analz_subset_parts";
-val parts_analz = thm "parts_analz";
-val analz_parts = thm "analz_parts";
-val analz_insertI = thm "analz_insertI";
-val Fake_parts_insert = thm "Fake_parts_insert";
-val Fake_analz_insert = thm "Fake_analz_insert";
+structure MessageSET =
+struct
 
 (*Prove base case (subgoal i) and simplify others.  A typical base case
   concerns  Crypt K X \<notin> Key`shrK`bad  and cannot be proved by rewriting
@@ -859,9 +854,9 @@ fun prove_simple_subgoals_tac i =
   Y \<in> parts(insert X H)  and  Y \<in> analz(insert X H)
 *)
 val Fake_insert_tac =
-    dresolve_tac [impOfSubs Fake_analz_insert,
-                  impOfSubs Fake_parts_insert] THEN'
-    eresolve_tac [asm_rl, thm"synth.Inj"];
+    dresolve_tac [impOfSubs @{thm Fake_analz_insert},
+                  impOfSubs @{thm Fake_parts_insert}] THEN'
+    eresolve_tac [asm_rl, @{thm synth.Inj}];
 
 fun Fake_insert_simp_tac ss i =
     REPEAT (Fake_insert_tac i) THEN asm_full_simp_tac ss i;
@@ -870,8 +865,8 @@ fun atomic_spy_analz_tac (cs,ss) = SELECT_GOAL
     (Fake_insert_simp_tac ss 1
      THEN
      IF_UNSOLVED (Blast.depth_tac
-		  (cs addIs [analz_insertI,
-				   impOfSubs analz_subset_parts]) 4 1))
+		  (cs addIs [@{thm analz_insertI},
+				   impOfSubs @{thm analz_subset_parts}]) 4 1))
 
 (*The explicit claset and simpset arguments help it work with Isar*)
 fun gen_spy_analz_tac (cs,ss) i =
@@ -887,6 +882,8 @@ fun gen_spy_analz_tac (cs,ss) i =
        DEPTH_SOLVE (atomic_spy_analz_tac (cs,ss) 1)]) i)
 
 fun spy_analz_tac i = gen_spy_analz_tac (claset(), simpset()) i
+
+end
 *}
 (*>*)
 
@@ -938,17 +935,17 @@ lemmas Fake_parts_sing_imp_Un = Fake_parts_sing [THEN [2] rev_subsetD]
 
 method_setup spy_analz = {*
     Method.ctxt_args (fn ctxt =>
-        Method.SIMPLE_METHOD' (gen_spy_analz_tac (local_clasimpset_of ctxt))) *}
+        Method.SIMPLE_METHOD' (MessageSET.gen_spy_analz_tac (local_clasimpset_of ctxt))) *}
     "for proving the Fake case when analz is involved"
 
 method_setup atomic_spy_analz = {*
     Method.ctxt_args (fn ctxt =>
-        Method.SIMPLE_METHOD' (atomic_spy_analz_tac (local_clasimpset_of ctxt))) *}
+        Method.SIMPLE_METHOD' (MessageSET.atomic_spy_analz_tac (local_clasimpset_of ctxt))) *}
     "for debugging spy_analz"
 
 method_setup Fake_insert_simp = {*
     Method.ctxt_args (fn ctxt =>
-        Method.SIMPLE_METHOD' (Fake_insert_simp_tac (local_simpset_of ctxt))) *}
+        Method.SIMPLE_METHOD' (MessageSET.Fake_insert_simp_tac (local_simpset_of ctxt))) *}
     "for debugging spy_analz"
 
 end
